fv: poke at completeness

fv/lean/Ragu/Circuits/Core/AllocMul.lean
@@ -10,29 +10,67 @@ structure Row (F : Type) where
 deriving ProvableStruct
 
 
-def main (_input : Unit) : Circuit (F p) (Var Row (F p)) := do
-  let ⟨x, y, z⟩ ← (witness fun _env => default : Circuit (F p) (Var Row (F p)))
+def main (w : Row (F p)) (_input : Unit) : Circuit (F p) (Var Row (F p)) := do
+  let ⟨x, y, z⟩ ← (witness fun _env => w : Circuit (F p) (Var Row (F p)))
   assertZero (x*y - z)
   return ⟨x, y, z⟩
 
-def Assumptions (_inputs : Unit) := True
+def Assumptions (w : Row (F p)) (_inputs : Unit) := w.x * w.y = w.z
 
 def Spec (_inputsinputs : Unit) (out_point : Row (F p)) :=
   out_point.x * out_point.y = out_point.z
 
-instance elaborated : ElaboratedCircuit (F p) unit Row where
-  main
+instance elaborated (w : Row (F p)) : ElaboratedCircuit (F p) unit Row where
+  main := main w
   localLength _ := 3
 
-theorem soundness : Soundness (F p) elaborated Assumptions Spec := by
+theorem soundness (w : Row (F p)) : Soundness (F p) (elaborated w) (Assumptions w) Spec := by
   circuit_proof_start
   ring_nf at *
-  simp_all only [sub_eq_iff_eq_add, zero_add]
+  grind
 
-theorem completeness : Completeness (F p) elaborated Assumptions := by
-  sorry
+theorem completeness (w : Row (F p)) : Completeness (F p) (elaborated w) (Assumptions w) := by
+  circuit_proof_start
+  simp only [List.sum_cons, List.sum_nil, Nat.add_zero, Nat.reduceAdd] at h_env
+  have h0 := h_env 0
+  have h1 := h_env 1
+  have h2 := h_env 2
+  simp only [Fin.isValue, Fin.coe_ofNat_eq_mod, Nat.zero_mod, add_zero, toElements, components,
+    instProvableTypeField.eq_1, id_eq, ProvableStruct.combinedSize', List.map_cons, size,
+    List.map_nil, List.sum_cons, List.sum_nil, Nat.add_zero, Nat.reduceAdd,
+    ProvableStruct.combinedSize, toComponents, ProvableStruct.componentsToElements.eq_2,
+    ProvableStruct.componentsToElements, Vector.append_empty, Vector.append_singleton,
+    Vector.push_mk, List.push_toArray, List.cons_append, List.nil_append, Vector.cast_rfl] at h0
+  rw [Vector.getElem_append] at h0
+  simp only [zero_lt_one, ↓reduceDIte, Vector.getElem_mk, List.getElem_toArray,
+    List.getElem_cons_zero] at h0
+  simp only [Fin.isValue, Fin.coe_ofNat_eq_mod, toElements, components, instProvableTypeField.eq_1,
+    id_eq, ProvableStruct.combinedSize', List.map_cons, size, List.map_nil, List.sum_cons,
+    List.sum_nil, Nat.add_zero, Nat.reduceAdd, ProvableStruct.combinedSize, toComponents,
+    ProvableStruct.componentsToElements.eq_2, ProvableStruct.componentsToElements,
+    Vector.append_empty, Vector.append_singleton, Vector.push_mk, List.push_toArray,
+    List.cons_append, List.nil_append, Vector.cast_rfl] at h1
+  rw [Vector.getElem_append] at h1
+  simp only [Nat.one_mod, lt_self_iff_false, ↓reduceDIte, tsub_self, Vector.getElem_mk,
+    List.getElem_toArray, List.getElem_cons_zero] at h1
+  simp only [Fin.isValue, Fin.coe_ofNat_eq_mod, toElements, components, instProvableTypeField.eq_1,
+    id_eq, ProvableStruct.combinedSize', List.map_cons, size, List.map_nil, List.sum_cons,
+    List.sum_nil, Nat.add_zero, Nat.reduceAdd, ProvableStruct.combinedSize, toComponents,
+    ProvableStruct.componentsToElements.eq_2, ProvableStruct.componentsToElements,
+    Vector.append_empty, Vector.append_singleton, Vector.push_mk, List.push_toArray,
+    List.cons_append, List.nil_append, Vector.cast_rfl] at h2
+  rw [Vector.getElem_append] at h2
+  simp only [Nat.mod_succ, Nat.not_ofNat_lt_one, ↓reduceDIte, Nat.add_one_sub_one,
+    Vector.getElem_mk, List.getElem_toArray, List.getElem_cons_succ, List.getElem_cons_zero] at h2
+  grind
 
-def circuit : FormalCircuit (F p) unit Row :=
-  { elaborated with Assumptions, Spec, soundness, completeness }
+def circuit (w : Row (F p)) : GeneralFormalCircuit (F p) unit Row :=
+  {
+    elaborated w with
+    Assumptions := Assumptions w,
+    Spec,
+    soundness := soundness w,
+    completeness := completeness w
+  }
 
 end Ragu.Circuits.Core.AllocMul
